{
 "cells": [
  {
   "cell_type": "markdown",
   "metadata": {},
   "source": [
    "$$\n",
    "\\begin{cases}\n",
    "u_t = \\Delta u + f\\\\\n",
    "u = g\n",
    "\\end{cases}\\\\\n",
    "\\rightarrow |u| \\leq e^{a |x|^2} + \\text{ conditions on } f, g\\\\\n",
    "\\rightarrow u = \\int \\Phi(x - y, t) g(y) dy + \\int_0^t \\int \\Phi(x - y, t - s) f(y, s) dy ds\\\\\n",
    "\\rightarrow\n",
    "\\begin{cases}\n",
    "u_t = \\Delta u\\\\\n",
    "u = g\n",
    "\\end{cases}\n",
    "$$\n",
    "\n",
    "Then since $g$ is bounded, we have $u \\in C^\\infty(R^n \\times (0, \\infty))$\n",
    "\n",
    "Sketch of proof:\n",
    "Box with $\\eta = 1$ inside box with $\\eta = 0$\n",
    "\n",
    "Then $v = \\nu u, v_t = \\Delta v + 2 \\nabla \\eta \\cdot \\nabla u + u \\Delta \\eta, v(x, 0) = 0$\n",
    "and\n",
    "$v(x, t) = \\int_0^t \\int (4 \\pi (t - s)) ^{-n / 2} e^{- \\frac{|x - y|^2}{4 (t - s)}} (2 \\nabla \\eta \\cdot \\nabla u + u \\Delta \\eta) \\in C^\\infty$"
   ]
  },
  {
   "cell_type": "markdown",
   "metadata": {},
   "source": [
    "So we've finished the heat equation, now we start with the wave equation.\n",
    "\n",
    "$$\n",
    "\\begin{cases}\n",
    "u_{tt} = \\Delta u + f(x, t), x \\in R^n\\\\\n",
    "u(x, 0) = g(x)\\\\\n",
    "u_t(x, 0) = h(x)\n",
    "\\end{cases}\n",
    "$$\n",
    "\n",
    "First we solve the simplest case, $n = 1, f = 0$\n",
    "We get\n",
    "\n",
    "$$\n",
    "\\begin{cases}\n",
    "u_{tt} = \\Delta u, x \\in R^n\\\\\n",
    "u(x, 0) = g(x)\\\\\n",
    "u_t(x, 0) = h(x)\n",
    "\\end{cases}\n",
    "$$\n",
    "\n",
    "d'Alembert's Formula\n",
    "\n",
    "1) Find general solutions to $u_{tt} - u_{xx} = 0$\\\\\n",
    "$\\partial^2_t - \\partial^2_x = (\\partial_t + \\partial_x) (\\partial_t - \\partial_x) = 0$\n",
    "\n",
    "\n",
    "From the characteristic curve idea from the transport equation we have\n",
    "$\\partial_\\zeta = \\partial_t + \\partial_x, \\partial_\\eta = \\partial_t - \\partial_x$\n",
    "$\\rightarrow \\partial_\\zeta(\\partial_\\eta u) = 0 \\rightarrow \\partial_\\eta u = f(\\eta)$\n",
    "\n",
    "Then\n",
    "$u = \\int f(\\eta) d \\eta + C(\\zeta) = F(\\zeta) + G(\\eta)$\n",
    "\n",
    "Much simpler than the heat and Laplace equations\n",
    "\n",
    "$$\n",
    "\\partial_\\zeta = \\partial_t + \\partial_x\\\\\n",
    "\\partial_\\eta = \\partial_t - \\partial_x\\\\\n",
    "\\rightarrow \\partial_t = \\frac{1}{2} \\partial_\\zeta + \\frac{1}{2} \\partial_\\eta\\\\\n",
    "\\partial_x = \\frac{1}{2} \\partial_\\zeta - \\frac{1}{2} \\partial_\\eta\\\\\n",
    "\\begin{pmatrix}\n",
    "\\partial_t\\\\\n",
    "\\partial_x\n",
    "\\end{pmatrix}\n",
    "=\n",
    "\\frac{1}{2}\n",
    "\\begin{pmatrix}\n",
    "1 & 1\\\\\n",
    "1 & -1\n",
    "\\end{pmatrix}\n",
    "\\begin{pmatrix}\n",
    "\\partial_\\zeta\\\\\n",
    "\\partial_\\eta\n",
    "\\end{pmatrix}\n",
    "$$\n",
    "Thus, our general solutions to $u_{tt} - u_{xx} = 0$ are $u(x, t) = F(x + t) + G(x - t)$\n",
    "\n",
    "2)\n",
    "Then\n",
    "$u(x, 0) = g(x) \\rightarrow F(x) + G(x) = g(x)$\n",
    "$u_t(x, 0) = h(x) \\rightarrow F'(x) - G'(x) = h(x)$\n",
    "\n",
    "$F(x) = \\frac{1}{2} \\left( g(x) + \\int_0^x h + A_0 \\right)$\\\\\n",
    "$G(x) = \\frac{1}{2} \\left( g(x) - \\int_0^x h - A_0 \\right)$\n",
    "\n",
    "$u = \\frac{1}{2} (g(x + t) + g(x - t)) + \\frac{1}{2} \\int_{x - t}^{x + t} h(y) dy$"
   ]
  },
  {
   "cell_type": "markdown",
   "metadata": {},
   "source": [
    "## Theorem 1\n",
    "\n",
    "$$\n",
    "u_{tt} = u_{xx}\\\\\n",
    "u(x, 0) = g(x),\\\\\n",
    "u_t(x, 0) = h(x)\n",
    "$$\n",
    "the solution above works for $n = 1$\n",
    "\n",
    "### Remark\n",
    "1) $g \\in C^k, h \\in C^{k - 1} \\rightarrow u \\in C^k$, so we have a loss of regularity compared to the heat and Laplace equations which are in $C^\\infty$. Discontinuities are propogated.\n",
    "2) $g, h = 0$ in $|x| \\geq R \\rightarrow u(x, t) = 0, |x| \\geq R + t$"
   ]
  },
  {
   "cell_type": "markdown",
   "metadata": {},
   "source": [
    "Next step, $n = 3$\n",
    "\n",
    "$$\n",
    "\\begin{cases}\n",
    "u_{tt} = \\Delta u\\\\\n",
    "u(x, 0) = g(x)\\\\\n",
    "u_t(x, 0) = h(x)\n",
    "\\end{cases}\n",
    "$$\n",
    "\n",
    "#### Trick 1\n",
    "Average. Fix $x_0 \\in R^3$\n",
    "\n",
    "Then\n",
    "$U(r, t) = \\frac{1}{|\\partial B_r(x_0) |} \\int_{\\partial  B_r(x_0)} u(y, t) dy$\n",
    "\n",
    "We claim that $U$ satisfies the wave equation\n",
    "\n",
    "$$\n",
    "U_{tt} = \\Delta U = U_{rr} + \\frac{2}{r} U_r\\\\\n",
    "u_{tt} = \\Delta u = u_{rr} + \\frac{2}{r} u_r + \\frac{\\Delta_S^2 u}{r^2}\\\\\n",
    "$$\n",
    "\n",
    "Averaging zeros out the Laplace-Beltrami operation, leaving us with our goal (this trick only works in $R^3$)\n",
    "\n",
    "Next\n",
    "$$\n",
    "\\begin{cases}\n",
    "U_{tt} = \\Delta U = U_{rr} + \\frac{2}{r} U_r\\\\\n",
    "U(r, 0) = \\bar{g}\\\\\n",
    "U_t(r, 0) = \\bar{h}\\\\\n",
    "\\bar{g} = \\frac{1}{|\\partial B_r(x_0)|} \\int_{\\partial B_r} g\n",
    "\\end{cases}\\\\\n",
    "\\tilde{U} = r U\\\\\n",
    "(r U)_{tt} = r U_{rr} + 2 U_{r} = (r U)_{rr} = r U_{rr} + 2 (r)' U_r + (r)'' U\n",
    "$$\n",
    "\n",
    "\n",
    "$$\n",
    "\\tilde{U}_{tt} = \\tilde{U}_{rr}\\\\\n",
    "\\tilde{U}(r, 0) = r \\bar{g}\\\\\n",
    "\\tilde{U}_t(r, 0) = r \\bar{h}\\\\\n",
    "\\tilde{U}(0, t) = 0\n",
    "$$\n",
    "\n",
    "Idea is to use the method of reflection\n",
    "\n",
    "$$\n",
    "\\tilde{g} =\n",
    "\\begin{cases}\n",
    "r \\bar{g} & r > 0\\\\\n",
    "-r \\bar{g}(-r) & r < 0\n",
    "\\end{cases}\\\\\n",
    "\\tilde{h} =\n",
    "\\begin{cases}\n",
    "\\bar{h} & r > 0\\\\\n",
    "-r \\bar{h}(-r) & r < 0\n",
    "\\end{cases}\n",
    "$$\n",
    "\n",
    "Then apply d'Alembert's Formula\n",
    "$$\n",
    "\\tilde{U}(r, t) = \\frac{1}{2} (\\tilde{g}(r + t) + \\tilde{g}(r - t)) + \\frac{1}{2} \\int_{r - t}^{r + t} \\tilde{h}(y) dy\n",
    "$$"
   ]
  },
  {
   "cell_type": "markdown",
   "metadata": {},
   "source": [
    "$$\n",
    "r U(r, t) = \\frac{1}{2} (\\tilde{g}(r + t) + \\tilde{g}(r - t)) + \\frac{1}{2} \\int_{r - t}^{r + t} \\tilde{h}(y) dy\n",
    "$$\n",
    "\n",
    "If $r > t$, we get\n",
    "$$\n",
    "r U(r, t) = \\frac{1}{2} ((r + t)\\bar{g}(r + t) + (r - t)\\bar{g}(r - t)) + \\frac{1}{2} \\int_{r - t}^{r + t} y \\bar{h}(y) dy\n",
    "$$\n",
    "This isn't what we want...\n",
    "\n",
    "If $r < t$, we get\n",
    "$$\n",
    "r U(r, t) = \\frac{1}{2} ((r + t)\\bar{g}(r + t) + (r - t)\\bar{g}(t - r)) + \\frac{1}{2} \\int_{0}^{r + t} y \\bar{h}(y) dy + \\frac{1}{2} \\int_{r - t}^{0} y \\bar{h}(-y) dy\n",
    "$$\n",
    "\n",
    "Then in total we have\n",
    "\n",
    "$$\n",
    "U(r, t) = \\frac{1}{2 r} ((r + t)\\bar{g}(r + t) + (r - t)\\bar{g}(t - r)) + \\frac{1}{2 r} \\int_{t - r}^{t + r} y \\bar{h}(y) dy\n",
    "$$\n"
   ]
  },
  {
   "cell_type": "markdown",
   "metadata": {},
   "source": [
    "Then since $U(r, t) = \\frac{1}{|\\partial B_r(x)|} \\int_{\\partial B_r(x)} u(t - r) d \\sigma$, as $r \\rightarrow 0$, we get $u(x, t) = t \\bar{h}(t) + \\bar{g}(t) + t \\bar{g}'(t) = \\frac{1}{2} (\\bar{g}(r + t) + \\bar{g}(t - r)) + \\frac{t}{2 r} (\\bar{g}(r + t) - \\bar{g}(t - r)) \\rightarrow_{r \\rightarrow 0} \\bar{g}(t) + t \\bar{g}'(t)$\n",
    "\n",
    "$\\bar{h}(t) = \\frac{|\\partial B_t(x)|} \\int_{\\partial B_t(x)} h$\n",
    "\n",
    "$\\bar{g}(t) = \\frac{1}{|\\partial B_t(x)|} \\int_{\\partial B_t(x)} g = \\frac{1}{|s^2|} \\int_{s^2} g(x + t \\theta) d\\theta$\n",
    "\n"
   ]
  },
  {
   "cell_type": "markdown",
   "metadata": {},
   "source": [
    "For the last homework problem you can use this formula\n",
    "$$\n",
    "u(x, t) = \\int_{\\partial B_t(x)} (t h(y) + g(y) + \\nabla g(y) \\cdot (y - x)) d\\sigma_y\n",
    "$$"
   ]
  },
  {
   "cell_type": "markdown",
   "metadata": {},
   "source": []
  }
 ],
 "metadata": {
  "kernelspec": {
   "display_name": "Python 3",
   "language": "python",
   "name": "python3"
  },
  "language_info": {
   "codemirror_mode": {
    "name": "ipython",
    "version": 3
   },
   "file_extension": ".py",
   "mimetype": "text/x-python",
   "name": "python",
   "nbconvert_exporter": "python",
   "pygments_lexer": "ipython3",
   "version": "3.7.4"
  }
 },
 "nbformat": 4,
 "nbformat_minor": 2
}
